heap_lang/sugar.v
@@ -60,17 +60,20 @@ Implicit Types Q : val → iProp heap_lang Σ.
 
 (** Proof rules for the sugar *)
 Lemma wp_lam E x ef e v Q :
-  to_val e = Some v → ▷ wp E (subst ef x v) Q ⊑ wp E (App (Lam x ef) e) Q.
-Proof. intros. by rewrite -wp_rec ?subst_empty; eauto. Qed.
+  to_val e = Some v → ▷ wp E (gsubst ef x e) Q ⊑ wp E (App (Lam x ef) e) Q.
+Proof.
+  intros <-%of_to_val; rewrite -wp_rec ?to_of_val //.
+  by rewrite (gsubst_correct _ _ (RecV _ _ _)) subst_empty.
+Qed.
 
 Lemma wp_let E x e1 e2 v Q :
-  to_val e1 = Some v → ▷ wp E (subst e2 x v) Q ⊑ wp E (Let x e1 e2) Q.
+  to_val e1 = Some v → ▷ wp E (gsubst e2 x e1) Q ⊑ wp E (Let x e1 e2) Q.
 Proof. apply wp_lam. Qed.
 
 Lemma wp_seq E e1 e2 Q : wp E e1 (λ _, ▷ wp E e2 Q) ⊑ wp E (Seq e1 e2) Q.
 Proof.
   rewrite -(wp_bind [LetCtx "" e2]). apply wp_mono=>v.
-  by rewrite -wp_let //= ?subst_empty ?to_of_val.
+  by rewrite -wp_let //= ?gsubst_correct ?subst_empty ?to_of_val.
 Qed.
 
 Lemma wp_le E (n1 n2 : nat) P Q :
